FSetEqProperties.v
@@ -27,425 +27,255 @@ Require Import Sumbool.
 Require Import Omega.
 
 Module EqProperties (M:S).
-  Import M.
-  Import Logic. (* to unmask [eq] *)  
-  Import Peano. (* to unmask [lt] *)
+Import M.
+Import Logic. (* to unmask [eq] *)  
+Import Peano. (* to unmask [lt] *)
   
-  Module ME := OrderedTypeFacts E.  
-  Module MP := Properties M.
-  Import MP.
-  Import MP.FM.
+Module ME := OrderedTypeFacts E.  
+Module MP := Properties M.
+Import MP.
+Import MP.FM.
 
-  Definition Add := MP.Add.
+Definition Add := MP.Add.
 
-  Section Old_Spec_Now_Properties. 
+Section BasicProperties. 
 
-  (** Other old specifications written with boolean equalities. *) 
+(** Some old specifications written with boolean equalities. *) 
 
-  Variable s s' : t.
-  Variable x y z : elt.
+Variable s s' s'': t.
+Variable x y z : elt.
 
-  Lemma mem_eq: 
-    E.eq x y -> mem x s=mem y s.
-  Proof. 
-  intro H; rewrite H; auto.
-  Qed.
+Lemma mem_eq: 
+  E.eq x y -> mem x s=mem y s.
+Proof. 
+intro H; rewrite H; auto.
+Qed.
 
-  Lemma equal_mem_1: 
-    (forall a, mem a s=mem a s') -> equal s s'=true.
-  Proof. 
-  intros; apply equal_1; unfold Equal; intros.
-  do 2 rewrite mem_iff; rewrite H; tauto.
-  Qed.
+Lemma equal_mem_1: 
+  (forall a, mem a s=mem a s') -> equal s s'=true.
+Proof. 
+intros; apply equal_1; unfold Equal; intros.
+do 2 rewrite mem_iff; rewrite H; tauto.
+Qed.
 
-  Lemma equal_mem_2: 
-    equal s s'=true -> forall a, mem a s=mem a s'.
-  Proof. 
-  intros; rewrite (equal_2 H); auto.
-  Qed.
+Lemma equal_mem_2: 
+  equal s s'=true -> forall a, mem a s=mem a s'.
+Proof. 
+intros; rewrite (equal_2 H); auto.
+Qed.
 
-  Lemma subset_mem_1: 
-    (forall a, mem a s=true->mem a s'=true) -> subset s s'=true.
-  Proof. 
-  intros; apply subset_1; unfold Subset; intros a.
-  do 2 rewrite mem_iff; auto.
-  Qed.
+Lemma subset_mem_1: 
+  (forall a, mem a s=true->mem a s'=true) -> subset s s'=true.
+Proof. 
+intros; apply subset_1; unfold Subset; intros a.
+do 2 rewrite mem_iff; auto.
+Qed.
 
-  Lemma subset_mem_2: 
-    subset s s'=true -> forall a, mem a s=true -> mem a s'=true.
-  Proof. 
-  intros H a; do 2 rewrite <- mem_iff; apply subset_2; auto.
-  Qed.
+Lemma subset_mem_2: 
+  subset s s'=true -> forall a, mem a s=true -> mem a s'=true.
+Proof. 
+intros H a; do 2 rewrite <- mem_iff; apply subset_2; auto.
+Qed.
   
-  Lemma empty_mem: mem x empty=false.
-  Proof. 
-  rewrite <- not_mem_iff; auto.
-  Qed.
+Lemma empty_mem: mem x empty=false.
+Proof. 
+rewrite <- not_mem_iff; auto.
+Qed.
 
-  Lemma is_empty_equal_empty: is_empty s = equal s empty.
-  Proof. 
-  apply bool_1; split; intros.
-  rewrite <- (empty_is_empty_1 (s:=empty)); auto with set.
-  rewrite <- is_empty_iff; auto with set.
-  Qed.
+Lemma is_empty_equal_empty: is_empty s = equal s empty.
+Proof. 
+apply bool_1; split; intros.
+rewrite <- (empty_is_empty_1 (s:=empty)); auto with set.
+rewrite <- is_empty_iff; auto with set.
+Qed.
   
-  Lemma choose_mem_1: choose s=Some x -> mem x s=true.
-  Proof.  
-  auto.
-  Qed.
+Lemma choose_mem_1: choose s=Some x -> mem x s=true.
+Proof.  
+auto.
+Qed.
 
-  Lemma choose_mem_2: choose s=None -> is_empty s=true.
-  Proof.
-  auto.
-  Qed.
+Lemma choose_mem_2: choose s=None -> is_empty s=true.
+Proof.
+auto.
+Qed.
 
-  Lemma add_mem_1: mem x (add x s)=true.
-  Proof.
-  auto.
-  Qed.  
+Lemma add_mem_1: mem x (add x s)=true.
+Proof.
+auto.
+Qed.  
  
-  Lemma add_mem_2: 
-  ~ E.eq x y -> mem y (add x s)=mem y s.
-  Proof. 
-  apply add_neq_b.
-  Qed.
+Lemma add_mem_2: ~E.eq x y -> mem y (add x s)=mem y s.
+Proof. 
+apply add_neq_b.
+Qed.
 
-  Lemma remove_mem_1: mem x (remove x s)=false.
-  Proof. 
-  rewrite <- not_mem_iff; auto.
-  Qed. 
+Lemma remove_mem_1: mem x (remove x s)=false.
+Proof. 
+rewrite <- not_mem_iff; auto.
+Qed. 
  
-  Lemma remove_mem_2: 
-  ~ E.eq x y -> mem y (remove x s)=mem y s.
-  Proof. 
-  apply remove_neq_b.
-  Qed.
+Lemma remove_mem_2: ~E.eq x y -> mem y (remove x s)=mem y s.
+Proof. 
+apply remove_neq_b.
+Qed.
 
-  Lemma singleton_equal_add: 
-    equal (singleton x) (add x empty)=true.
-  Proof.
-  rewrite (singleton_equal_add x); auto with set.
-  Qed.  
+Lemma singleton_equal_add: 
+  equal (singleton x) (add x empty)=true.
+Proof.
+rewrite (singleton_equal_add x); auto with set.
+Qed.  
 
-  Lemma union_mem: 
-    mem x (union s s')=mem x s || mem x s'.
-  Proof. 
-  apply union_b.
-  Qed.
+Lemma union_mem: 
+  mem x (union s s')=mem x s || mem x s'.
+Proof. 
+apply union_b.
+Qed.
 
-  Lemma inter_mem: 
-    mem x (inter s s')=mem x s && mem x s'.
-  Proof. 
-  apply inter_b.
-  Qed.
+Lemma inter_mem: 
+  mem x (inter s s')=mem x s && mem x s'.
+Proof. 
+apply inter_b.
+Qed.
 
-  Lemma diff_mem: 
-    mem x (diff s s')=mem x s && negb (mem x s').
-  Proof. 
-  apply diff_b.
-  Qed.
-
-  Section fold. 
-
-  Variable A:Set. 
-  Variable eqA:A->A->Prop.
-  Variable st:Setoid_Theory _ eqA.
-  Variable i:A.
-  Variable f:elt->A->A.
-  Variable Comp:compat_op E.eq eqA f. 
-  Variable Assoc:transpose eqA f.
- 
-  Lemma fold_empty: eqA (fold f empty i) i.
-  Proof. 
-  apply fold_empty; auto.
-  Qed.
-
-  Lemma fold_equal: 
-    equal s s'=true -> eqA (fold f s i) (fold f s' i).
-  Proof. 
-  intros; apply fold_equal with (eqA:=eqA); auto.
-  Qed.
-   
-  Lemma fold_add: 
-    mem x s=false -> eqA (fold f (add x s) i) (f x (fold f s i)).
-  Proof. 
-    intros; apply fold_add with (eqA:=eqA); auto.
-    rewrite not_mem_iff; auto.
-  Qed.
-
-  End fold.
-
-  Section Filter.
-  
-  Variable f:elt->bool.
-  Variable Comp: compat_bool E.eq f.
-
-  Lemma filter_mem: mem x (filter f s)=mem x s && f x.
-  Proof. 
-  apply filter_b; auto.
-  Qed.
-
-  Lemma for_all_filter: 
-    for_all f s=is_empty (filter (fun x => negb (f x)) s).
-  Proof. 
-  assert (Comp' : compat_bool E.eq (fun x =>negb (f x))). 
-    generalize Comp; unfold compat_bool; intros; f_equal; auto. 
-  apply bool_1; split; intros.
-  apply is_empty_1.
-  unfold Empty; intros. 
-  rewrite filter_iff; auto.
-  red; destruct 1.
-  rewrite <- (@for_all_iff s f) in H; auto.
-  rewrite (H a H0) in H1; discriminate.
-  apply for_all_1; auto; red; intros.
-  revert H; rewrite <- is_empty_iff.
-  unfold Empty; intro H; generalize (H x0); clear H.
-  rewrite filter_iff; auto.
-  destruct (f x0); auto.
-  Qed.
-
-  Lemma exists_filter : 
-    exists_ f s=negb (is_empty (filter f s)).
-  Proof. 
-  apply bool_1; split; intros. 
-  destruct (exists_2 Comp H) as (a,(Ha1,Ha2)).
-  apply bool_6.
-  red; intros; apply (@is_empty_2 _ H0 a); auto.
-  generalize (@choose_1 (filter f s)) (@choose_2 (filter f s)).
-  destruct (choose (filter f s)).
-  intros H0 _; apply exists_1; auto.
-  exists e; generalize (H0 e); rewrite filter_iff; auto.
-  intros _ H0.
-  rewrite (is_empty_1 (H0 (refl_equal None))) in H; auto; discriminate.
-  Qed.
-
-  Lemma partition_filter_1: 
-     equal (fst (partition f s)) (filter f s)=true.
-  Proof. 
-  auto.
-  Qed.
-
-  Lemma partition_filter_2: 
-     equal (snd (partition f s)) (filter (fun x => negb (f x)) s)=true.
-  Proof. 
-  auto.
-  Qed.
-
-  End Filter.
-  End Old_Spec_Now_Properties.
-
-  Hint Immediate empty_mem is_empty_equal_empty add_mem_1
-    remove_mem_1 singleton_equal_add union_mem inter_mem
-    diff_mem filter_mem for_all_filter exists_filter : set. 
-  Hint Resolve equal_mem_1 subset_mem_1 choose_mem_1
-    choose_mem_2 add_mem_2 remove_mem_2 : set.
-
-Section MoreProperties.
+Lemma diff_mem: 
+  mem x (diff s s')=mem x s && negb (mem x s').
+Proof. 
+apply diff_b.
+Qed.
 
 (** properties of [mem] *)
 
-Lemma mem_3 : forall s x, ~In x s -> mem x s=false.
+Lemma mem_3 : ~In x s -> mem x s=false.
 Proof.
 intros; rewrite <- not_mem_iff; auto.
 Qed.
 
-Lemma mem_4 : forall s x, mem x s=false -> ~In x s.
+Lemma mem_4 : mem x s=false -> ~In x s.
 Proof.
 intros; rewrite not_mem_iff; auto.
 Qed.
 
 (** Properties of [equal] *) 
 
-Lemma equal_refl: forall s, equal s s=true.
+Lemma equal_refl: equal s s=true.
 Proof.
 auto with set.
 Qed.
 
-Lemma equal_sym: forall s s', equal s s'=equal s' s.
+Lemma equal_sym: equal s s'=equal s' s.
 Proof.
 intros; apply bool_1; do 2 rewrite <- equal_iff; intuition.
 Qed.
 
 Lemma equal_trans: 
- forall s u v, equal s u=true -> equal u v=true -> equal s v=true.
+ equal s s'=true -> equal s' s''=true -> equal s s''=true.
 Proof.
 intros; rewrite (equal_2 H); auto.
 Qed.
 
 Lemma equal_equal: 
- forall s s' s'', equal s s'=true -> equal s s''=equal s' s''.
+ equal s s'=true -> equal s s''=equal s' s''.
 Proof.
 intros; rewrite (equal_2 H); auto.
 Qed.
 
 Lemma equal_cardinal: 
- forall s s', equal s s'=true -> cardinal s=cardinal s'.
+ equal s s'=true -> cardinal s=cardinal s'.
 Proof.
-intros; rewrite (equal_2 H); auto.
+auto with set.
 Qed.
-
-Hint Resolve equal_refl equal_cardinal equal_equal:set.
-Hint Immediate equal_sym :set.
 
 (* Properties of [subset] *)
 
-Lemma subset_refl: forall s, subset s s=true. 
+Lemma subset_refl: subset s s=true. 
 Proof.
 auto with set.
 Qed.
 
 Lemma subset_antisym: 
- forall s s', subset s s'=true -> subset s' s=true -> equal s s'=true.
+ subset s s'=true -> subset s' s=true -> equal s s'=true.
 Proof.
-intros s s'; do 2 rewrite <- subset_iff; rewrite <- equal_iff.
-apply subset_antisym.
+auto with set.
 Qed.
 
 Lemma subset_trans: 
- forall s s' s'', subset s s'=true -> subset s' s''=true -> subset s s''=true.
+ subset s s'=true -> subset s' s''=true -> subset s s''=true.
 Proof.
-intros s s' s''; do 3 rewrite <- subset_iff; intros.
+do 3 rewrite <- subset_iff; intros.
 apply subset_trans with s'; auto.
 Qed.
 
 Lemma subset_equal: 
- forall s s', equal s s'=true -> subset s s'=true.
+ equal s s'=true -> subset s s'=true.
 Proof.
-intros; rewrite (equal_2 H); auto with set.
+auto with set.
 Qed.
-
-Hint Resolve subset_refl subset_equal subset_antisym :set.
 
 (** Properties of [choose] *)
 
 Lemma choose_mem_3: 
- forall s, is_empty s=false -> {x:elt|choose s=Some x /\ mem x s=true}.
+ is_empty s=false -> {x:elt|choose s=Some x /\ mem x s=true}.
 Proof.
 intros.
-generalize (@choose_mem_1 s) (@choose_mem_2 s).
-case (choose s);intros.
+generalize (@choose_1 s) (@choose_2 s).
+destruct (choose s);intros.
 exists e;auto.
-lapply H1;trivial;intros.
-rewrite H in H2;discriminate H2.
+generalize (H1 (refl_equal None)); clear H1.
+intros; rewrite (is_empty_1 H1) in H; discriminate.
 Qed.
 
 Lemma choose_mem_4: choose empty=None.
 Proof.
-generalize (@choose_mem_1 empty).
+generalize (@choose_1 empty).
 case (@choose empty);intros;auto.
-absurd (true=false);auto with bool.
-rewrite <- (H e);auto with set.
+elim (@empty_1 e); auto.
 Qed.
 
 (** Properties of [add] *)
 
 Lemma add_mem_3: 
- forall s x y, mem y s=true -> mem y (add x s)=true.
+ mem y s=true -> mem y (add x s)=true.
 Proof.
 auto.
 Qed.
 
 Lemma add_equal: 
- forall s x, mem x s=true -> equal (add x s) s=true.
-Proof.
-intros s x; rewrite <- mem_iff; intros; apply equal_1; auto with set.
-Qed.
-
-Hint Resolve add_mem_3 add_equal :set.
-
-Lemma add_fold: 
- forall (A:Set)(eqA:A->A->Prop)(st:(Setoid_Theory _ eqA))
- (f:elt->A->A)(i:A), (compat_op E.eq eqA f) -> (transpose eqA f) ->
- forall (s:t)(x:elt), mem x s=true -> (eqA (fold f (add x s) i) (fold f s i)).
-Proof.
-intros; apply fold_equal with (eqA:=eqA); auto with set.
-Qed.
-
-Lemma add_cardinal_1: 
- forall s x, mem x s=true -> cardinal (add x s)=cardinal s.
+ mem x s=true -> equal (add x s) s=true.
 Proof.
 auto with set.
-Qed.
-
-Lemma add_cardinal_2: 
- forall s x, mem x s=false -> cardinal (add x s)=S (cardinal s).
-Proof.
-intros.
-do 2 rewrite MP.cardinal_fold.
-change S with ((fun _ =>S) x); apply fold_add with (eqA:=@eq nat); auto.
 Qed.
 
 (** Properties of [remove] *)
 
 Lemma remove_mem_3: 
- forall s x y, mem y (remove x s)=true -> mem y s=true.
+ mem y (remove x s)=true -> mem y s=true.
 Proof.
-intros s x y; rewrite remove_b; intros H;destruct (andb_prop _ _ H); auto.
+rewrite remove_b; intros H;destruct (andb_prop _ _ H); auto.
 Qed.
 
 Lemma remove_equal: 
- forall s x, mem x s=false -> equal (remove x s) s=true.
+ mem x s=false -> equal (remove x s) s=true.
 Proof.
 intros; apply equal_1; apply remove_equal.
-intro H0; rewrite (mem_1 H0) in H; discriminate.
+rewrite not_mem_iff; auto.
 Qed.
 
-Hint Resolve remove_mem_3 remove_equal : set.
-
 Lemma add_remove: 
- forall s x, mem x s=true -> equal (add x (remove x s)) s=true.
+ mem x s=true -> equal (add x (remove x s)) s=true.
 Proof.
 intros; apply equal_1; apply add_remove; auto.
 Qed.
 
 Lemma remove_add: 
- forall s x, mem x s=false -> equal (remove x (add x s)) s=true.
+ mem x s=false -> equal (remove x (add x s)) s=true.
 Proof.
 intros; apply equal_1; apply remove_add; auto.
-intro H0; rewrite (mem_1 H0) in H; discriminate.
-Qed.
-
-Hint Immediate add_remove remove_add : set.
-
-Lemma remove_fold_1: 
- forall (A:Set)(eqA:A->A->Prop)(st:(Setoid_Theory _ eqA))
- (f:elt->A->A)(i:A), (compat_op E.eq eqA f) -> (transpose eqA f) ->
- forall s x, mem x s=true -> 
- eqA (f x (fold f (remove x s) i)) (fold f s i).
-Proof.
-intros.
-apply Seq_sym; auto.
-apply MP.fold_2 with (eqA:=eqA); auto.
-Qed.
-
-Lemma remove_fold_2: 
- forall (A:Set)(eqA:A->A->Prop)(st:(Setoid_Theory _ eqA))
- (f:elt->A->A)(i:A), (compat_op E.eq eqA f) -> (transpose eqA f) ->
- forall s x, mem x s=false -> 
- eqA (fold f (remove x s) i) (fold f s i).
-Proof.
-intros.
-apply fold_equal with (eqA:=eqA); auto with set.
-Qed.
-
-Lemma remove_cardinal_1: 
- forall s x, mem x s=true -> S (cardinal (remove x s))=cardinal s.
-Proof.
-intros.
-do 2 rewrite cardinal_fold.
-change S with ((fun _ =>S) x).
-apply remove_fold_1 with (eqA:=@eq nat); auto.
-Qed.
-
-Lemma remove_cardinal_2: 
- forall s x, mem x s=false -> cardinal (remove x s)=cardinal s.
-Proof.
-auto with set.
+rewrite not_mem_iff; auto.
 Qed.
 
 (** Properties of [is_empty] *)
 
-Lemma is_empty_cardinal: forall s, is_empty s = zerob (cardinal s).
+Lemma is_empty_cardinal: is_empty s = zerob (cardinal s).
 Proof.
 intros; apply bool_1; split; intros.
 rewrite cardinal_1; simpl; auto.
@@ -455,23 +285,203 @@ Qed.
 
 (** Properties of [singleton] *)
 
-Lemma singleton_mem_1: forall x, mem x (singleton x)=true.
+Lemma singleton_mem_1: mem x (singleton x)=true.
 Proof.
-intros; apply mem_1; auto.
+auto with set.
 Qed.
 
-Lemma singleton_mem_2: forall x y, ~E.eq x y -> mem y (singleton x)=false.
+Lemma singleton_mem_2: ~E.eq x y -> mem y (singleton x)=false.
 Proof.
 intros; rewrite singleton_b.
 unfold ME.eqb; destruct (ME.eq_dec x y); intuition.
 Qed.
 
-Lemma singleton_mem_3: forall x y, mem y (singleton x)=true -> E.eq x y.
+Lemma singleton_mem_3: mem y (singleton x)=true -> E.eq x y.
 Proof.
 auto.
 Qed.
 
-(* General recursion principes based on [cardinal] *)
+(** Properties of [union] *)
+
+Lemma union_sym:
+ equal (union s s') (union s' s)=true.
+Proof.
+auto with set.
+Qed.
+
+Lemma union_subset_equal: 
+ subset s s'=true -> equal (union s s') s'=true.
+Proof.
+auto with set.
+Qed.
+
+Lemma union_equal_1: 
+ equal s s'=true-> equal (union s s'') (union s' s'')=true.
+Proof.
+auto with set.
+Qed.
+
+Lemma union_equal_2: 
+ equal s' s''=true-> equal (union s s') (union s s'')=true.
+Proof.
+auto with set.
+Qed.
+
+Lemma union_assoc: 
+ equal (union (union s s') s'') (union s (union s' s''))=true.
+Proof.
+auto with set.
+Qed.
+
+Lemma add_union_singleton: 
+ equal (add x s) (union (singleton x) s)=true.
+Proof.
+auto with set.
+Qed.
+
+Lemma union_add: 
+ equal (union (add x s) s') (add x (union s s'))=true.
+Proof.
+auto with set.
+Qed.
+
+(* caracterisation of [union] via [subset] *)
+
+Lemma union_subset_1: subset s (union s s')=true.
+Proof.
+auto with set.
+Qed.
+
+Lemma union_subset_2: subset s' (union s s')=true.
+Proof.
+auto with set.
+Qed.
+
+Lemma union_subset_3:
+ subset s s''=true -> subset s' s''=true -> 
+  subset (union s s') s''=true.
+Proof.
+intros; apply subset_1; apply union_subset_3; auto.
+Qed.
+
+(** Properties of [inter] *) 
+
+Lemma inter_sym: equal (inter s s') (inter s' s)=true.
+Proof.
+auto with set.
+Qed.
+
+Lemma inter_subset_equal: 
+ subset s s'=true -> equal (inter s s') s=true.
+Proof.
+auto with set.
+Qed.
+
+Lemma inter_equal_1: 
+ equal s s'=true -> equal (inter s s'') (inter s' s'')=true.
+Proof.
+auto with set.
+Qed.
+
+Lemma inter_equal_2: 
+ equal s' s''=true -> equal (inter s s') (inter s s'')=true.
+Proof.
+auto with set.
+Qed.
+
+Lemma inter_assoc: 
+ equal (inter (inter s s') s'') (inter s (inter s' s''))=true.
+Proof.
+auto with set.
+Qed.
+
+Lemma union_inter_1: 
+ equal (inter (union s s') s'') (union (inter s s'') (inter s' s''))=true.
+Proof.
+auto with set.
+Qed.
+
+Lemma union_inter_2: 
+ equal (union (inter s s') s'') (inter (union s s'') (union s' s''))=true.
+Proof.
+auto with set.
+Qed.
+
+Lemma inter_add_1: mem x s'=true -> 
+ equal (inter (add x s) s') (add x (inter s s'))=true.
+Proof.
+auto with set.
+Qed.
+
+Lemma inter_add_2: mem x s'=false -> 
+ equal (inter (add x s) s') (inter s s')=true.
+Proof.
+intros; apply equal_1; apply inter_add_2.
+rewrite not_mem_iff; auto.
+Qed.
+
+(* caracterisation of [union] via [subset] *)
+
+Lemma inter_subset_1: subset (inter s s') s=true.
+Proof.
+auto with set.
+Qed.
+
+Lemma inter_subset_2: subset (inter s s') s'=true.
+Proof.
+auto with set.
+Qed.
+
+Lemma inter_subset_3:
+ subset s'' s=true -> subset s'' s'=true -> 
+  subset s'' (inter s s')=true.
+Proof.
+intros; apply subset_1; apply inter_subset_3; auto.
+Qed.
+
+(** Properties of [diff] *)
+
+Lemma diff_subset: subset (diff s s') s=true.
+Proof.
+auto with set.
+Qed.
+
+Lemma diff_subset_equal:
+ subset s s'=true -> equal (diff s s') empty=true.
+Proof.
+auto with set.
+Qed.
+
+Lemma remove_inter_singleton: 
+ equal (remove x s) (diff s (singleton x))=true.
+Proof.
+auto with set.
+Qed.
+
+Lemma diff_inter_empty:
+ equal (inter (diff s s') (inter s s')) empty=true. 
+Proof.
+auto with set.
+Qed.
+
+Lemma diff_inter_all: 
+ equal (union (diff s s') (inter s s')) s=true.
+Proof.
+auto with set.
+Qed.
+
+End BasicProperties.
+
+Hint Immediate empty_mem is_empty_equal_empty add_mem_1
+   remove_mem_1 singleton_equal_add union_mem inter_mem
+   diff_mem equal_sym add_remove remove_add : set. 
+Hint Resolve equal_mem_1 subset_mem_1 choose_mem_1
+   choose_mem_2 add_mem_2 remove_mem_2 equal_refl equal_equal
+   subset_refl subset_equal subset_antisym
+   add_mem_3 add_equal remove_mem_3 remove_equal : set.
+
+
+(** General recursion principes based on [cardinal] *)
 
 Lemma cardinal_set_rec:  forall (P:t->Type),
  (forall s s', equal s s'=true -> P s -> P s') -> 
@@ -494,171 +504,7 @@ Proof.
 intros;apply cardinal_set_rec with (cardinal s);auto.
 Qed.
 
-(** Properties of [union] *)
-
-Lemma union_sym:
- forall s s', equal (union s s') (union s' s)=true.
-Proof.
-intros;apply equal_1;apply union_sym. 
-Qed.
-
-Lemma union_subset_equal: 
- forall s s', subset s s'=true -> equal (union s s') s'=true.
-Proof.
-intros; apply equal_1; apply union_subset_equal; auto.
-Qed.
-
-Lemma union_equal_1: 
- forall s s' s'', equal s s'=true->
- equal (union s s'') (union s' s'')=true.
-Proof.
-intros; apply equal_1; apply union_equal_1; auto.
-Qed.
-
-Lemma union_equal_2: 
- forall s s' s'', equal s' s''=true->
- equal (union s s') (union s s'')=true.
-Proof.
-intros;apply equal_1;apply union_equal_2; auto.
-Qed.
-
-Lemma union_assoc: 
- forall s s' s'',
- equal (union (union s s') s'') (union s (union s' s''))=true.
-Proof.
-intros;apply equal_1;apply union_assoc; auto.
-Qed.
-
-Lemma add_union_singleton: 
- forall s x, equal (add x s) (union (singleton x) s)=true.
-Proof.
-intros;apply equal_1;apply add_union_singleton.
-Qed.
-
-Lemma union_add: 
- forall s s' x,
- equal (union (add x s) s') (add x (union s s'))=true.
-Proof.
-intros;apply equal_1;apply union_add.
-Qed.
-
-(* caracterisation of [union] via [subset] *)
-
-Lemma union_subset_1:
- forall s s',(subset s (union s s'))=true.
-Proof.
-intros;apply subset_mem_1;intros;rewrite union_mem;rewrite H;auto.
-Qed.
-
-Lemma union_subset_2:
- forall s s',(subset s' (union s s'))=true.
-Proof.
-intros;apply subset_mem_1;intros;rewrite union_mem;rewrite H;apply orb_b_true.
-Qed.
-
-Lemma union_subset_3:
- forall s s' s'', (subset s s'')=true -> (subset s' s'')=true -> 
-    (subset (union s s') s'')=true.
-Proof.
-intros;apply subset_mem_1;intros;rewrite union_mem in H1.
-elim (orb_true_elim _ _ H1);intros.
-apply (subset_mem_2 _ _ H _ a0).
-apply (subset_mem_2 _ _ H0 _ b).
-Qed.
-
-(** Properties of [inter] *) 
-
-Lemma inter_sym:
- forall s s',(equal (inter s s') (inter s' s))=true.
-Proof.
-intros;apply equal_mem_1;intros.
-do 2 rewrite inter_mem.
-auto with bool.
-Qed.
-
-Lemma inter_subset_equal: 
- forall s s',(subset s s')=true->(equal (inter s s') s)=true.
-Proof.
-intros.
-apply equal_mem_1;intros.
-rewrite inter_mem.
-apply (bool_eq_ind (mem a s));intros;simpl;auto.
-rewrite (subset_mem_2 _ _ H _ H0);auto.
-Qed.
-
-Lemma inter_equal_1: 
- forall s s' s'', equal s s'=true->
- equal (inter s s'') (inter s' s'')=true.
-Proof.
-intros s s' s''; do 2 rewrite <- equal_iff; apply inter_equal_1.
-Qed.
-
-Lemma inter_equal_2: 
- forall s s' s'', equal s' s''=true->
- equal (inter s s') (inter s s'')=true.
-Proof.
-intros s s' s''; do 2 rewrite <- equal_iff; apply inter_equal_2.
-Qed.
-
-Lemma inter_assoc: 
- forall s s' s'',
- equal (inter (inter s s') s'') (inter s (inter s' s''))=true.
-Proof.
-intros; apply equal_1; apply inter_assoc.
-Qed.
-
-Lemma union_inter_1: 
- forall s s' s'',
- equal (inter (union s s') s'') (union (inter s s'') (inter s' s''))=true.
-Proof.
-intros;apply equal_1;apply union_inter_1.
-Qed.
-
-Lemma union_inter_2: 
- forall s s' s'',
- equal (union (inter s s') s'') (inter (union s s'') (union s' s''))=true.
-Proof.
-intros; apply equal_1; apply union_inter_2.
-Qed.
-
-Lemma inter_add_1: 
- forall s s' x, mem x s'=true -> 
- equal (inter (add x s) s') (add x (inter s s'))=true.
-Proof.
-intros; apply equal_1; apply inter_add_1; auto with set.
-Qed.
-
-Lemma inter_add_2: 
- forall s s' x, mem x s'=false -> 
- equal (inter (add x s) s') (inter s s')=true.
-Proof.
-intros; apply equal_1; apply inter_add_2.
-rewrite not_mem_iff; auto.
-Qed.
-
-(* caracterisation of [union] via [subset] *)
-
-Lemma inter_subset_1:
- forall s s',(subset (inter s s') s)=true.
-Proof.
-intros;apply subset_mem_1;intros;rewrite inter_mem in H;elim (andb_prop _ _ H);auto.
-Qed.
-
-Lemma inter_subset_2:
- forall s s',(subset (inter s s') s')=true.
-Proof.
-intros;apply subset_mem_1;intros;rewrite inter_mem in H;elim (andb_prop _ _ H);auto.
-Qed.
-
-Lemma inter_subset_3:
- forall s s' s'',(subset s'' s)=true -> (subset s'' s')=true -> 
-    (subset s'' (inter s s'))=true.
-intros;apply subset_mem_1;intros;rewrite inter_mem.
-rewrite (subset_mem_2 _ _ H _ H1);
-rewrite (subset_mem_2 _ _ H0 _ H1);auto.
-Qed.
-
-(** Properties of [union],[inter],[fold] and [cardinal] *)
+(** Properties of [fold] *)
 
 Lemma exclusive_set : forall s s' x,
  ~In x s\/~In x s' <-> mem x s && mem x s'=false.
@@ -667,14 +513,84 @@ intros; do 2 rewrite not_mem_iff.
 destruct (mem x s); destruct (mem x s'); intuition.
 Qed.
 
-Lemma fold_union: 
- forall (A:Set)(f:elt->A->A)(i:A), 
- compat_op E.eq (@eq A) f -> transpose (@eq A) f -> 
- forall s s', (forall x, mem x s && mem x s'=false) -> 
- fold f (union s s') i = fold f s (fold f s' i).
+Section Fold. 
+Variables (A:Set)(eqA:A->A->Prop)(st:Setoid_Theory _ eqA).
+Variables (f:elt->A->A)(Comp:compat_op E.eq eqA f)(Ass:transpose eqA f).
+Variables (i:A).
+Variables (s s':t)(x:elt).
+ 
+Lemma fold_empty: eqA (fold f empty i) i.
+Proof. 
+apply fold_empty; auto.
+Qed.
+
+Lemma fold_equal: 
+ equal s s'=true -> eqA (fold f s i) (fold f s' i).
+Proof. 
+intros; apply fold_equal with (eqA:=eqA); auto.
+Qed.
+   
+Lemma fold_add: 
+ mem x s=false -> eqA (fold f (add x s) i) (f x (fold f s i)).
+Proof. 
+intros; apply fold_add with (eqA:=eqA); auto.
+rewrite not_mem_iff; auto.
+Qed.
+
+Lemma add_fold: 
+  mem x s=true -> eqA (fold f (add x s) i) (fold f s i).
 Proof.
-intros; apply fold_union; auto; intros.
-rewrite exclusive_set; auto.
+intros; apply add_fold with (eqA:=eqA); auto.
+Qed.
+
+Lemma remove_fold_1: 
+ mem x s=true -> eqA (f x (fold f (remove x s) i)) (fold f s i).
+Proof.
+intros; apply remove_fold_1 with (eqA:=eqA); auto.
+Qed.
+
+Lemma remove_fold_2: 
+ mem x s=false -> eqA (fold f (remove x s) i) (fold f s i).
+Proof.
+intros; apply remove_fold_2 with (eqA:=eqA); auto.
+rewrite not_mem_iff; auto.
+Qed.
+
+Lemma fold_union: 
+ (forall x, mem x s && mem x s'=false) -> 
+ eqA (fold f (union s s') i) (fold f s (fold f s' i)).
+Proof.
+intros; apply fold_union with (eqA:=eqA); auto.
+intros; rewrite exclusive_set; auto.
+Qed.
+
+End Fold.
+
+(** Properties of [cardinal] *)
+
+Lemma add_cardinal_1: 
+ forall s x, mem x s=true -> cardinal (add x s)=cardinal s.
+Proof.
+auto with set.
+Qed.
+
+Lemma add_cardinal_2: 
+ forall s x, mem x s=false -> cardinal (add x s)=S (cardinal s).
+Proof.
+intros; apply add_cardinal_2; auto.
+rewrite not_mem_iff; auto.
+Qed.
+
+Lemma remove_cardinal_1: 
+ forall s x, mem x s=true -> S (cardinal (remove x s))=cardinal s.
+Proof.
+intros; apply remove_cardinal_1; auto.
+Qed.
+
+Lemma remove_cardinal_2: 
+ forall s x, mem x s=false -> cardinal (remove x s)=cardinal s.
+Proof.
+auto with set.
 Qed.
 
 Lemma union_cardinal: 
@@ -685,105 +601,120 @@ intros; apply union_cardinal; auto; intros.
 rewrite exclusive_set; auto.
 Qed.
 
-(** Properties of [diff] *)
-
-Lemma diff_subset: 
- forall s s', subset (diff s s') s=true.
-Proof.
-intros.
-apply subset_mem_1;intros.
-rewrite diff_mem in H.
-elim (andb_prop _ _ H);auto.
-Qed.
-
-Lemma diff_subset_equal:
- forall s s', subset s s'=true -> equal (diff s s') empty=true.
-Proof.
-intros.
-apply equal_mem_1;intros.
-rewrite empty_mem.
-rewrite diff_mem.
-generalize (@subset_mem_2 _ _ H a).
-case (mem a s);simpl;intros;auto.
-rewrite H0;auto.
-Qed.
-
-Lemma remove_inter_singleton: 
- forall s x, equal (remove x s) (diff s (singleton x))=true.
-Proof.
-intros;apply equal_mem_1;intros.
-rewrite diff_mem.
-elim (ME.eq_dec x a); intros.
-rewrite <- (mem_eq (remove x s) _ _ a0).
-rewrite <- (mem_eq s _ _ a0).
-rewrite <- (mem_eq (singleton x) _ _ a0).
-rewrite remove_mem_1;rewrite singleton_mem_1;rewrite andb_b_false;auto.
-rewrite singleton_mem_2;auto;simpl;rewrite andb_b_true;auto with set.
-Qed.
-
-Lemma diff_inter_empty:
- forall s s', equal (inter (diff s s') (inter s s')) empty=true. 
-Proof.
-intros; apply equal_1; apply diff_inter_empty; auto.
-Qed.
-
-Lemma diff_inter_all: 
-forall s s', equal (union (diff s s') (inter s s')) s=true.
-Proof.
-intros; apply equal_1; apply diff_inter_all; auto.
-Qed.
-
-Lemma diff_inter_cardinal: 
- forall s s',(cardinal (diff s s'))+(cardinal (inter s s'))=(cardinal s).
-Proof.
-intros.
-do 3 rewrite MP.cardinal_fold.
-rewrite <- fold_plus.
-apply fold_diff_inter; auto.
-Qed.
-
 Lemma subset_cardinal: 
  forall s s', subset s s'=true -> cardinal s<=cardinal s'.
 Proof.
-intros.
-rewrite <- (diff_inter_cardinal s' s).
-rewrite (equal_cardinal _ _ (inter_sym s' s)).
-rewrite (equal_cardinal _ _ (inter_subset_equal _ _ H)); auto with arith.
+intros; apply subset_cardinal; auto.
+Qed.
+
+Section Bool.
+
+(** Properties of [filter] *)
+
+Variable f:elt->bool.
+Variable Comp: compat_bool E.eq f.
+
+Let Comp' : compat_bool E.eq (fun x =>negb (f x)).
+Proof.
+unfold compat_bool in *; intros; f_equal; auto.
+Qed.
+
+Lemma filter_mem: forall s x, mem x (filter f s)=mem x s && f x.
+Proof. 
+intros; apply filter_b; auto.
+Qed.
+
+Lemma for_all_filter: 
+ forall s, for_all f s=is_empty (filter (fun x => negb (f x)) s).
+Proof. 
+intros; apply bool_1; split; intros.
+apply is_empty_1.
+unfold Empty; intros. 
+rewrite filter_iff; auto.
+red; destruct 1.
+rewrite <- (@for_all_iff s f) in H; auto.
+rewrite (H a H0) in H1; discriminate.
+apply for_all_1; auto; red; intros.
+revert H; rewrite <- is_empty_iff.
+unfold Empty; intro H; generalize (H x); clear H.
+rewrite filter_iff; auto.
+destruct (f x); auto.
+Qed.
+
+Lemma exists_filter : 
+ forall s, exists_ f s=negb (is_empty (filter f s)).
+Proof. 
+intros; apply bool_1; split; intros. 
+destruct (exists_2 Comp H) as (a,(Ha1,Ha2)).
+apply bool_6.
+red; intros; apply (@is_empty_2 _ H0 a); auto.
+generalize (@choose_1 (filter f s)) (@choose_2 (filter f s)).
+destruct (choose (filter f s)).
+intros H0 _; apply exists_1; auto.
+exists e; generalize (H0 e); rewrite filter_iff; auto.
+intros _ H0.
+rewrite (is_empty_1 (H0 (refl_equal None))) in H; auto; discriminate.
+Qed.
+
+Lemma partition_filter_1: 
+ forall s, equal (fst (partition f s)) (filter f s)=true.
+Proof. 
+auto.
+Qed.
+
+Lemma partition_filter_2: 
+ forall s, equal (snd (partition f s)) (filter (fun x => negb (f x)) s)=true.
+Proof. 
+auto.
+Qed.
+
+Lemma add_filter_1 : forall s s' x, 
+ f x=true -> (Add x s s') -> (Add x (filter f s) (filter f s')).
+Proof.
+unfold Add, MP.Add; intros.
+repeat rewrite filter_iff; auto.
+rewrite H0; clear H0.
+assert (E.eq x y -> f y = true) by 
+ intro H0; rewrite <- (Comp _ _ H0); auto.
+tauto.
+Qed.
+
+Lemma add_filter_2 : forall s s' x, 
+ f x=false -> (Add x s s') -> filter f s [=] filter f s'.
+Proof.
+unfold Add, MP.Add, Equal; intros.
+repeat rewrite filter_iff; auto.
+rewrite H0; clear H0.
+assert (f a = true -> ~E.eq x a).
+ intros H0 H1.
+ rewrite (Comp _ _ H1) in H.
+ rewrite H in H0; discriminate.
+tauto. 
 Qed.
 
 (** Properties of [for_all] *)
 
-Section For_all.
-
-Variable f : elt->bool.
-Variable Comp : (compat_bool E.eq f).
-
-Let Comp' : (compat_bool E.eq (fun x =>negb (f x))).
-Proof.
-generalize Comp; unfold compat_bool; intros; apply (f_equal negb);auto.
-Qed.
-
-Lemma for_all_mem_1: 
- forall s, (forall x, (mem x s)=true->(f x)=true) -> (for_all f s)=true.
+Lemma for_all_mem_1: forall s, 
+ (forall x, (mem x s)=true->(f x)=true) -> (for_all f s)=true.
 Proof.
 intros.
 rewrite for_all_filter; auto.
 rewrite is_empty_equal_empty.
 apply equal_mem_1;intros.
-rewrite filter_mem; auto.
+rewrite filter_b; auto.
 rewrite empty_mem.
 generalize (H a); case (mem a s);intros;auto.
 rewrite H0;auto.
 Qed.
 
-Lemma for_all_mem_2: 
- forall s, (for_all f s)=true -> forall x,(mem x s)=true -> (f x)=true. 
+Lemma for_all_mem_2: forall s, 
+ (for_all f s)=true -> forall x,(mem x s)=true -> (f x)=true. 
 Proof.
 intros.
 rewrite for_all_filter in H; auto.
 rewrite is_empty_equal_empty in H.
 generalize (equal_mem_2 _ _ H x).
-rewrite filter_mem; auto.
+rewrite filter_b; auto.
 rewrite empty_mem.
 rewrite H0; simpl;intros.
 replace true with (negb false);auto;apply negb_sym;auto.
@@ -797,7 +728,7 @@ apply (bool_eq_ind (for_all f s));intros;auto.
 rewrite for_all_filter in H1; auto.
 rewrite is_empty_equal_empty in H1.
 generalize (equal_mem_2 _ _ H1 x).
-rewrite filter_mem; auto.
+rewrite filter_b; auto.
 rewrite empty_mem.
 rewrite H.
 rewrite H0.
@@ -805,48 +736,43 @@ simpl;auto.
 Qed.
 
 Lemma for_all_mem_4: 
- forall s, (for_all f s)=false -> {x:elt | (mem x s)=true /\ (f x)=false}.
+ forall s, for_all f s=false -> {x:elt | mem x s=true /\ f x=false}.
+Proof.
 intros.
 rewrite for_all_filter in H; auto.
-elim (choose_mem_3 _ H);intros;elim p;intros.
+destruct (choose_mem_3 _ H) as (x,(H0,H1));intros.
 exists x.
-rewrite filter_mem in H1; auto.
+rewrite filter_b in H1; auto.
 elim (andb_prop _ _ H1).
 split;auto.
 replace false with (negb true);auto;apply negb_sym;auto.
 Qed.
 
-End For_all.
-
 (** Properties of [exists] *)
 
-Section exists_.
-
-Variable f : elt->bool.
-Variable Comp : (compat_bool E.eq f).
-
-Let Comp' : (compat_bool E.eq (fun x => negb (f x))).
-Proof.
-generalize Comp; unfold compat_bool; intros; apply (f_equal negb);auto.
-Qed.
-
 Lemma for_all_exists: 
- forall s, (exists_ f s)=(negb (for_all (fun x =>negb (f x)) s)).
+ forall s, exists_ f s = negb (for_all (fun x =>negb (f x)) s).
 Proof.
 intros.
-rewrite for_all_filter; auto.
-rewrite exists_filter; auto.
-apply (f_equal negb).
-do 2 rewrite is_empty_equal_empty.
-apply equal_equal.
-apply equal_mem_1;intros.
-do 2 (rewrite filter_mem; auto).
-rewrite negb_elim;auto.
-generalize Comp'; unfold compat_bool; intros; apply (f_equal negb); auto.
+rewrite for_all_b; auto.
+rewrite exists_b; auto.
+induction (elements s); simpl; auto.
+destruct (f a); simpl; auto.
+Qed.
+
+End Bool.
+Section Bool'.
+
+Variable f:elt->bool.
+Variable Comp: compat_bool E.eq f.
+
+Let Comp' : compat_bool E.eq (fun x =>negb (f x)).
+Proof.
+unfold compat_bool in *; intros; f_equal; auto.
 Qed.
 
 Lemma exists_mem_1: 
- forall s, (forall x, (mem x s)=true->(f x)=false) -> (exists_ f s)=false.
+ forall s, (forall x, mem x s=true->f x=false) -> exists_ f s=false.
 Proof.
 intros.
 rewrite for_all_exists; auto.
@@ -856,30 +782,30 @@ symmetry;apply negb_sym;simpl;auto.
 Qed.
 
 Lemma exists_mem_2: 
- forall s, (exists_ f s)=false -> forall x, (mem x s)=true -> (f x)=false. 
+ forall s, exists_ f s=false -> forall x, mem x s=true -> f x=false. 
 Proof.
 intros.
-rewrite for_all_exists in H.
+rewrite for_all_exists in H; auto.
 replace false with (negb true);auto;apply negb_sym;symmetry.
 rewrite (for_all_mem_2 (fun x => negb (f x)) Comp' s);simpl;auto.
 replace true with (negb false);auto;apply negb_sym;auto.
 Qed.
 
 Lemma exists_mem_3: 
- forall s x,(mem x s)=true -> (f x)=true -> (exists_ f s)=true.
+ forall s x, mem x s=true -> f x=true -> exists_ f s=true.
 Proof.
 intros.
-rewrite for_all_exists.
+rewrite for_all_exists; auto.
 symmetry;apply negb_sym;simpl.
 apply for_all_mem_3 with x;auto.
 rewrite H0;auto.
 Qed.
 
 Lemma exists_mem_4: 
- forall s, (exists_ f s)=true -> {x:elt | (mem x s)=true /\ (f x)=true}.
+ forall s, exists_ f s=true -> {x:elt | (mem x s)=true /\ (f x)=true}.
 Proof.
 intros.
-rewrite for_all_exists in H.
+rewrite for_all_exists in H; auto.
 elim (for_all_mem_4 (fun x =>negb (f x)) Comp' s);intros.
 elim p;intros.
 exists x;split;auto.
@@ -887,16 +813,15 @@ replace true with (negb false);auto;apply negb_sym;auto.
 replace false with (negb true);auto;apply negb_sym;auto.
 Qed.
 
-End exists_.
+End Bool'.
 
 Section Sum.
-
 
 Definition sum (f:elt -> nat)(s:t) := fold (fun x => plus (f x)) s 0. 
 
 Lemma sum_plus : 
-  forall f g, (compat_nat E.eq f) -> (compat_nat E.eq g) -> 
-    forall s, (sum (fun x =>(f x)+(g x)) s) = (sum f s)+(sum g s).
+  forall f g, compat_nat E.eq f -> compat_nat E.eq g -> 
+    forall s, sum (fun x =>f x+g x) s = sum f s + sum g s.
 Proof.
 unfold sum.
 intros f g Hf Hg.
@@ -909,60 +834,20 @@ assert (fgt : transpose (@eq _) (fun x:elt=>plus ((f x)+(g x)))). red; intros; o
 assert (st := gen_st nat).
 intros s;pattern s; apply set_rec.
 intros.
-rewrite <- (fold_equal _ _ _ _ st O _ fc ft H).
-rewrite <- (fold_equal _ _ _ _ st O _ gc gt H).
-rewrite <- (fold_equal _ _ _ _ st O _ fgc fgt H); auto.
-assert (fold_add' := fun s t =>(fold_add s t _ _ st)).
-intros; do 3 (rewrite fold_add';auto).
+rewrite <- (fold_equal _ _ st _ fc ft 0 _ _ H).
+rewrite <- (fold_equal _ _ st _ gc gt 0 _ _ H).
+rewrite <- (fold_equal _ _ st _ fgc fgt 0 _ _ H); auto.
+intros; do 3 (rewrite (fold_add _ _ st);auto).
 rewrite H0;simpl;omega.
 intros; do 3 rewrite (fold_empty _ _ st);auto.
 Qed.
 
-Lemma filter_equal : forall f, (compat_bool E.eq f) -> 
-     forall s s',(Equal s s') -> (Equal (filter f s) (filter f s')).
-Proof.
-unfold Equal; split; intros; elim (H0 a); intros; apply filter_3; eauto.
-Qed.
-
-Lemma add_filter_1 : forall f, (compat_bool E.eq f) -> 
-  forall s s' x, (f x)=true -> (Add x s s') -> (Add x (filter f s) (filter f s')).
-Proof.
-unfold Add; split; intros; elim (H1 y); clear H1; intros.
-elim H1; [ auto | right; eauto | eauto ].
-apply filter_3; auto.
-elim H2; intros.
-intuition.
-apply H3; right; eauto.
-elim H2; intros.
-rewrite <- H0; auto.
-eauto.
-Qed.
-
-Lemma add_filter_2 :  forall f, (compat_bool E.eq f) -> 
-  forall s s' x, (f x)=false -> (Add x s s') -> (Equal (filter f s) (filter f s')).
-Proof.
-unfold Add, Equal; split; intros; elim (H1 a); clear H1; intros.
-elim H1; intros. 
-absurd (true=false); auto with bool.
-rewrite <- H0. 
-rewrite <- (filter_2 H H2); auto.
-apply filter_3; eauto.
-apply H3; right; eauto.
-
-elim H1; intros. 
-absurd (true=false); auto with bool.
-rewrite <- H0. 
-rewrite <- (filter_2 H H2); auto.
-eauto.
-eauto.
-Qed.
 
 Lemma sum_filter : forall f, (compat_bool E.eq f) -> 
   forall s, (sum (fun x => if f x then 1 else 0) s) = (cardinal (filter f s)).
 Proof.
 unfold sum; intros f Hf.
 assert (st := gen_st nat).
-assert (fold_add' := fun s t => fold_add s t _ _ st).
 assert (cc : compat_op E.eq (@eq _) (fun x => plus (if f x then 1 else 0))). 
  unfold compat_op; intros.
  rewrite (Hf x x' H); auto.
@@ -971,9 +856,9 @@ assert (ct : transpose (@eq _) (fun x => plus (if f x then 1 else 0))).
 intros s;pattern s; apply set_rec.
 intros.
 change elt with E.t.
-rewrite <- (fold_equal _ _ _ _ st O _ cc ct H).
-rewrite <- (MP.Equal_cardinal (filter_equal _ Hf _ _ (equal_2 H))); auto.
-intros; rewrite fold_add'; auto.
+rewrite <- (fold_equal _ _ st _ cc ct 0 _ _ H).
+rewrite <- (MP.Equal_cardinal (filter_equal Hf (equal_2 H))); auto.
+intros; rewrite (fold_add _ _ st _ cc ct); auto.
 generalize (@add_filter_1 f Hf s0 (add x s0) x) (@add_filter_2 f Hf s0 (add x s0) x) .
 assert (~ In x (filter f s0)).
  intro H1; rewrite (mem_1 (filter_1 Hf H1)) in H; discriminate H.
@@ -1014,8 +899,8 @@ apply (Seq_trans _ _ st) with i; [idtac | apply Seq_sym; auto]; apply fold_empty
 Qed.
 
 Lemma sum_compat : 
-  forall f g, (compat_nat E.eq f) -> (compat_nat E.eq g) -> 
-  forall s, (forall x, (In x s) -> (f x)=(g x)) -> (sum f s)=(sum g s).
+  forall f g, compat_nat E.eq f -> compat_nat E.eq g -> 
+  forall s, (forall x, In x s -> f x=g x) -> sum f s=sum g s.
 intros.
 unfold sum; apply (fold_compat _ (@eq nat)); auto.
 unfold transpose; intros; omega.
@@ -1024,8 +909,8 @@ Qed.
 
 End Sum.
 
-Lemma filter_orb: forall f g, (compat_bool E.eq f) -> (compat_bool E.eq g) ->
-  forall s, (Equal (filter (fun x=>orb (f x) (g x)) s) (union (filter f s) (filter g s))).
+Lemma union_filter: forall f g, (compat_bool E.eq f) -> (compat_bool E.eq g) ->
+  forall s, union (filter f s) (filter g s) [=] filter (fun x=>orb (f x) (g x)) s.
 Proof.
 intros.
 assert (compat_bool E.eq (fun x => orb (f x) (g x))).
@@ -1033,14 +918,12 @@ assert (compat_bool E.eq (fun x => orb (f x) (g x))).
   rewrite (H x y H1).
   rewrite (H0 x y H1); auto.
 unfold Equal; split; intros.
-assert (H3 := filter_1 H1 H2).
-assert (H4 := filter_2 H1 H2).
-elim (orb_prop _ _ H4); intros; eauto.
 elim (union_1 H2); intros. 
 apply filter_3; [ auto | eauto | rewrite (filter_2 H H3); auto ].
 apply filter_3; [ auto | eauto | rewrite (filter_2 H0 H3); auto with bool].
+assert (H3 := filter_1 H1 H2).
+assert (H4 := filter_2 H1 H2).
+elim (orb_prop _ _ H4); intros; eauto.
 Qed.
-
-End MoreProperties.
 
 End EqProperties. 
